examples/MutableMap/MutableMapExamples.dfy
@@ -6,54 +6,40 @@
 // RUN: %dafny /compile:0 "%s"
 
 include "../../src/MutableMap/MutableMap.dfy"
-include "../../src/Wrappers.dfy"
 
 module {:options "-functionSyntax:4"} MutableMapExamples {
   import opened MutableMap
-  import opened Wrappers
 
-  method AssertAndExpect(p: bool, maybeMsg: Option<string> := None) requires p {
-    match maybeMsg {
-      case None => {
-          expect p;
-      }
-      case Some(msg) => {
-          expect p, msg;
-      }
-    }
-  }
-
-  method Main() 
-  {
-    var m := MutableMap<string,string>.Make();
-    AssertAndExpect(m.Keys() == {});
-    AssertAndExpect(m.Values() == {});
-    AssertAndExpect(m.Items() == {});
-    AssertAndExpect(m.Size() == 0);
+  method Main() {
+    var m := new MutableMap<string,string>();
+    assert m.Keys() == {};
+    assert m.Values() == {};
+    assert m.Items() == {};
+    assert m.Size() == 0;
     m.Put("testkey", "testvalue");
-    AssertAndExpect(m.Select("testkey") == "testvalue");
-    AssertAndExpect(m.Keys() == {"testkey"});
-    AssertAndExpect(m.Values() == {"testvalue"});
-    AssertAndExpect(m.Items() == {("testkey", "testvalue")});
-    AssertAndExpect(m.Size() == 1);
+    assert m.Select("testkey") == "testvalue";
+    assert m.Keys() == {"testkey"};
+    assert m.Values() == {"testvalue"};
+    assert m.Items() == {("testkey", "testvalue")};
+    assert m.Size() == 1;
     m.Put("testkey", "testvalue2");
-    AssertAndExpect(m.Keys() == {"testkey"});
-    AssertAndExpect(m.Values() == {"testvalue2"});
-    AssertAndExpect(m.Items() == {("testkey", "testvalue2")});
+    assert m.Keys() == {"testkey"};
+    assert m.Values() == {"testvalue2"};
+    assert m.Items() == {("testkey", "testvalue2")};
     m.Put("testkey2", "testvalue2");
-    AssertAndExpect(m.Keys() == {"testkey", "testkey2"});
-    AssertAndExpect(m.Values() == {"testvalue2"});
-    AssertAndExpect(m.Items() == {("testkey", "testvalue2"), ("testkey2", "testvalue2")});
-    AssertAndExpect(m.Size() == 2);
-    AssertAndExpect("testkey" in m.Keys());
-    AssertAndExpect("testkey2" in m.Keys());
+    assert m.Keys() == {"testkey", "testkey2"};
+    assert m.Values() == {"testvalue2"};
+    assert m.Items() == {("testkey", "testvalue2"), ("testkey2", "testvalue2")};
+    assert m.Size() == 2;
+    assert "testkey" in m.Keys();
+    assert "testkey2" in m.Keys();
     print m.Select("testkey"), "\n";
     print m.Select("testkey2"), "\n";
     m.Remove("testkey");
-    AssertAndExpect(m.SelectOpt("testkey").None?);
-    AssertAndExpect(m.SelectOpt("testkey2").Some? && m.SelectOpt("testkey2").value == "testvalue2");
-    AssertAndExpect(m.Keys() == {"testkey2"});
-    AssertAndExpect(m.Values() == {"testvalue2"});
-    AssertAndExpect(m.Items() == {("testkey2", "testvalue2")});
+    assert m.SelectOpt("testkey").None?;
+    assert m.SelectOpt("testkey2").Some? && m.SelectOpt("testkey2").value == "testvalue2";
+    assert m.Keys() == {"testkey2"};
+    assert m.Values() == {"testvalue2"};
+    assert m.Items() == {("testkey2", "testvalue2")};
   }
 }
